Updated bounded operators

QHoare.thy
@@ -15,10 +15,10 @@ definition "ifthen R x = R (butterket x x)" for R :: \<open>'a update \<Rightarr
 definition "program S = fold (o\<^sub>C\<^sub>L) S idOp" for S :: \<open>'mem update list\<close>
 
 
-definition hoare :: \<open>'mem ell2 clinear_space \<Rightarrow> ('mem ell2 \<Rightarrow>\<^sub>C\<^sub>L 'mem ell2) list \<Rightarrow> 'mem ell2 clinear_space \<Rightarrow> bool\<close> where
+definition hoare :: \<open>'mem ell2 ccsubspace \<Rightarrow> ('mem ell2 \<Rightarrow>\<^sub>C\<^sub>L 'mem ell2) list \<Rightarrow> 'mem ell2 ccsubspace \<Rightarrow> bool\<close> where
   "hoare C p D \<longleftrightarrow> (\<forall>\<psi>\<in>space_as_set C. program p *\<^sub>V \<psi> \<in> space_as_set D)" for C p D
 
-definition EQ :: "('a update \<Rightarrow> 'mem update) \<Rightarrow> 'a ell2 \<Rightarrow> 'mem ell2 clinear_space" (infix "=\<^sub>q" 75) where
+definition EQ :: "('a update \<Rightarrow> 'mem update) \<Rightarrow> 'a ell2 \<Rightarrow> 'mem ell2 ccsubspace" (infix "=\<^sub>q" 75) where
   "EQ R \<psi> = R (selfbutter \<psi>) *\<^sub>S \<top>"
 
 lemma program_skip[simp]: "program [] = idOp"
@@ -34,21 +34,21 @@ lemma hoare_seq[trans]: "hoare C p1 D \<Longrightarrow> hoare D p2 E \<Longright
 
 lemma hoare_weaken_left[trans]: \<open>A \<le> B \<Longrightarrow> hoare B p C \<Longrightarrow> hoare A p C\<close>
   unfolding hoare_def
-  by (meson in_mono less_eq_clinear_space.rep_eq) 
+  by (meson in_mono less_eq_ccsubspace.rep_eq) 
 
 lemma hoare_weaken_right[trans]: \<open>hoare A p B \<Longrightarrow> B \<le> C \<Longrightarrow> hoare A p C\<close>
   unfolding hoare_def 
-  by (meson in_mono less_eq_clinear_space.rep_eq) 
+  by (meson in_mono less_eq_ccsubspace.rep_eq) 
 
 lemma hoare_skip: "C \<le> D \<Longrightarrow> hoare C [] D"
-  by (auto simp: program_def hoare_def times_applyOp in_mono less_eq_clinear_space.rep_eq)
+  by (auto simp: program_def hoare_def times_applyOp in_mono less_eq_ccsubspace.rep_eq)
 
 lemma hoare_apply: 
   assumes "R U *\<^sub>S pre \<le> post"
   shows "hoare pre [apply U R] post"
   using assms 
   apply (auto simp: hoare_def program_def apply_def)
-  by (metis (no_types, lifting) applyOpSpace.rep_eq closure_subset imageI less_eq_clinear_space.rep_eq subsetD)
+  by (metis (no_types, lifting) applyOpSpace.rep_eq closure_subset imageI less_eq_ccsubspace.rep_eq subsetD)
 
 lemma hoare_ifthen: 
   fixes R :: \<open>'a update \<Rightarrow> 'mem update\<close>
@@ -56,7 +56,7 @@ lemma hoare_ifthen:
   shows "hoare pre [ifthen R x] post"
   using assms 
   apply (auto simp: hoare_def program_def ifthen_def butterfly_def')
-  by (metis (no_types, lifting) applyOpSpace.rep_eq closure_subset imageI less_eq_clinear_space.rep_eq subsetD)
+  by (metis (no_types, lifting) applyOpSpace.rep_eq closure_subset imageI less_eq_ccsubspace.rep_eq subsetD)
 
 end
 
